src/Prototype/Simulation.v
@@ -1,0 +1,77 @@
+Require Import Bool List String Peano_dec.
+Require Import FnMap Language.
+
+Section Simulation.
+  Context {MsgT StateT: Type}.
+  Local Notation State := (State MsgT StateT).
+
+  Variable sim: State -> State -> Prop.
+  Local Infix "≈" := sim (at level 30).
+
+  Variables impl spec: System MsgT StateT.
+
+  Definition Simulates :=
+    forall ist1 sst1,
+      ist1 ≈ sst1 ->
+      forall ilbl ist2,
+        step impl ist1 ilbl ist2 ->
+        match getBLabel impl ilbl with
+        | Some b =>
+          exists sst2 slbl, step spec sst1 slbl sst2 /\
+                            getBLabel spec slbl = Some b /\
+                            ist2 ≈ sst2
+        | None =>
+          (exists sst2 slbl, step spec sst1 slbl sst2 /\
+                             getBLabel spec slbl = None /\
+                             ist2 ≈ sst2) \/
+          ist2 ≈ sst1
+        end.
+
+  Hypothesis (Hsim: Simulates).
+
+  Lemma simulation_steps:
+    forall ist1 sst1,
+      ist1 ≈ sst1 ->
+      forall ihst ist2,
+        steps impl ist1 ihst ist2 ->
+        exists sst2 shst,
+          behaviorOf impl ihst = behaviorOf spec shst /\
+          steps spec sst1 shst sst2 /\
+          ist2 ≈ sst2.
+  Proof.
+    induction 2; simpl; intros;
+      [exists sst1, nil; repeat split; auto; constructor|].
+
+    specialize (IHsteps H).
+    destruct IHsteps as [sst2 [shst [? [? ?]]]].
+
+    eapply Hsim in H1; [|exact H4].
+    remember (getBLabel impl lbl) as blbl; destruct blbl as [blbl|]; simpl.
+
+    - destruct H1 as [sst3 [slbl [? [? ?]]]].
+      eexists; eexists (slbl :: _); repeat split; eauto.
+      + simpl; rewrite H2, H5; simpl; reflexivity.
+      + econstructor; eauto.
+    - destruct H1.
+      * destruct H1 as [sst3 [slbl [? [? ?]]]].
+        eexists; eexists (slbl :: _); repeat split; eauto.
+        -- simpl; rewrite H2, H5; simpl; reflexivity.
+        -- econstructor; eauto.
+      * exists sst2, shst; repeat split; auto.
+  Qed.
+
+  Hypothesis (Hsimi: sim {| st_oss := getObjectStatesInit impl; st_msgs := @empty _ _ |}
+                         {| st_oss := getObjectStatesInit spec; st_msgs := @empty _ _ |}).
+
+  Theorem simulation_implies_refinement:
+    Refines impl spec.
+  Proof.
+    unfold Simulates, Refines; intros.
+    inv H.
+    eapply simulation_steps in H0; [|exact Hsimi].
+    destruct H0 as [? [? [? [? ?]]]].
+    econstructor; eauto.
+  Qed.
+
+End Simulation.
+
